\documentclass[11pt]{article}

\title{ECO206 Microeconomic Theory\\ \small Second Degree Price Discrimination \small}
\author{Tianyu Du}
\date{\today}

\usepackage{spikey}
\usepackage{amsmath}
\usepackage{amssymb}

\begin{document}

	\maketitle
	
	\section{Setup}
	\paragraph{} Consider two groups of customers with different marginal willingness to pay. Their demands are captured by demand function
	\begin{equation}
		D_i = f_i (p)\ i \in \{L, H\}
	\end{equation}
	Assuming $H$ group has higher MWTP at any quantity of $x$, that's 
	\begin{equation}
		f_H^{-1}(x) > f_L^{-1}(x) \ \forall x \in \R_+
	\end{equation}
	Let function $C_L(x)$ and $C_H(x)$ denote the cost to provide goods/services to each group of customer.
	\\
	Define welfare function for customers
	\begin{equation}
		u_i(x_i) = \int_{0}^{x_i} f_i^{-1}(x)\ dx \ i \in \{L, H\}
	\end{equation}
	By equation (2), we have
	\begin{equation}
		u_H(x) > u_L(x) \ \forall x \in \R_+
	\end{equation}

	\section{Mathematical Form}
	The profit optimization problem of producer can be formalized as
	\begin{equation}
		\max_{x_L,p_L,x_H,p_H} \big \{\pi(\cdot) =  P_L - C_L(x_L) + P_H - C_H(x_H) \big \}
	\end{equation} 
	subject to \underbar{individual rationality} and \underbar{intensive compatibility} constraints
	\begin{equation}
		\begin{cases}
			u_L(x_L) - p_L \geq 0 \\
			u_H(x_H) - p_H \geq 0 \\
			u_L(x_L) - p_L \geq u_L(x_H) - p_H \\
			u_H(x_H) - p_H \geq u_H(x_L) - p_L \\
		\end{cases}
	\end{equation}
	
	\section{Reduce the Constraint Region}
	The constraint can be reduced to
	\begin{equation}
		\begin{cases}
			u_L(x_L) - p_L = 0 \\
			u_L(x_H) - p_H \leq 0 \\
			u_H(x_H) - p_H = u_H(x_L) - p_L \\
		\end{cases}
	\end{equation}
	
	\section{Solving the Problem}
		We want to write $\pi(\cdot)$ as a function of $x_L$ and solve the optimal $x_L$.
	\subsection{Step 1: Directly solve $x_H^*$}
		We wish to sell \underbar{efficient amount} to the high types, that's where MC(supply) equals demand.
		Find $x_H^*$ by solving
		\begin{equation}
			\pd{C_H(x_H)}{x_H}\bigg\vert_{x_H = x_H^*} = f_H^{-1}(x_H^*)
		\end{equation}
	\subsection{Step 2: Rewrite $P_L$}
		Using equation (7.1), we can map $x_L$ to $p_L$ by
		\begin{equation}
			p_L(x_L) = u_L(x_L) = \int_0^{x_L} f_L^{-1}(x)\ dx
		\end{equation}
	\subsection{Step 3: Rewrite $p_H$}
		Using equation (7.3) to map $x_L$ to $p_H$ as
		\begin{equation}
			p_H(x_L) = \overline{u_H(x_H^*)} - \int_{0}^{x_L}f_H^{-1}(x)\ dx + p_L(x_L)
		\end{equation}
	\subsection{Step 4: Solving Problem}
		By equation (7.2)
		\begin{equation}
			p_H \geq u_L(x_H^*) \iff x_L \leq x_H^*
		\end{equation}
		\begin{multline*}
			\emph{Proof.} \\
			7.2 \implies u_L(x_H) \leq p_H \\
			\tx{(with 7.3)} \implies u_L(x_H) \leq u_H(x_H) - u_H(x_L) + p_L \\
			\implies u_L(x_H) \leq u_H(x_H) - u_H(x_L) + u_L(x_L) \\
			\implies u_L(x_H) - u_L(x_L) \leq u_H(x_H) - u_H(x_L) \\
			\implies \int_{x_L}^{x_H} f_L^{-1}(x)\ dx \leq \int_{x_L}^{x_H} f_H^{-1}(x)\ dx \\
			\tx{as } 0 < f_L^{-1}(x) < f_H^{-1}(x) \ \forall x \in \R_+ \\
			\iff x_L \leq x_H \\
			\blacksquare
		\end{multline*}
		Rewrite the objective function as 
		\begin{equation}
			\pi(x_L) = P_L(x_L) + P_H(x_L) - C_L(x_L) - \overline{C_H(x_H^*)}
		\end{equation}
		and maximize $\pi(x_L)$ by solving $\pd{\pi(x_L)}{x_L} = 0$ and $x_L \in [0, x_H^*)$.
\end{document}
























